more lemmas

VmSemantics.v
@@ -120,39 +120,6 @@ Definition run_vm (il:list AnnoInstr) st : vm_st :=
 Definition run_vm_t (t:AnnoTerm) st : vm_st :=
   run_vm (instr_compiler t) st.
 
-(*
-(** Relational-style semantics for VM *)
-Record vm_config : Type :=
-  mk_config
-    {vm_ev:EvidenceC ;
-     vm_list:list AnnoInstr ;
-      vm_stack:ev_stack
-    }.
-
-
-Inductive vm_step : vm_config -> vm_config -> (list Ev) -> Prop :=
-| do_vmStep : forall e i l s,
-    let res_st := execSt (mk_st e s []) (build_comp i) in
-    let e' := st_ev res_st in
-    let s' := st_stack res_st in
-    let tr' := st_trace res_st in
-    vm_step (mk_config e (i::l) s) (mk_config e' l s') tr'.
-
-Definition vm_multi : step_relation vm_config Ev := refl_trans_1n_trace vm_step.
-
-Lemma step_implies_multi : forall e e' i l tr s s',
-    vm_step (mk_config e (i::l) s) (mk_config e' l s') tr ->
-    vm_multi (mk_config e (i::l) s) (mk_config e' l s') tr.
-Proof.
-  intros.
-  cut (vm_multi {| vm_ev := e; vm_list := i :: l; vm_stack := s |}
-                   {| vm_ev := e'; vm_list := l; vm_stack := s' |} (tr++[])).
-  rewrite app_nil_r. auto.
-  repeat econstructor; eauto.
-Defined.
-Hint Resolve step_implies_multi.
-*)
-
 Lemma st_congr :
   forall st tr e s,
     st_ev st = e ->
@@ -221,50 +188,29 @@ Defined.
           pop_stackm {| st_ev := _; st_stack := _; st_trace := _|} |- _ ] => idtac "hello"; edestruct (pop_stackm_fail); eauto; clear H; destruct_conjs
     end; monad_unfold.
 
-Lemma trace_irrel : forall il1 tr1 tr1' tr2 e e' s s',
-
-    run_vm il1 {| st_ev := e; st_trace := tr1; st_stack := s |} =
-    {| st_ev := e'; st_trace := tr1'; st_stack := s' |} ->
-    
-    st_ev (
-        run_vm il1 {| st_ev := e; st_trace := tr2; st_stack := s |}) = e'.
-Proof.
-  induction il1; intros.
-  - simpl.
-    inversion H. reflexivity.
-    
-  -
-    simpl;
-    destruct a; try (destruct p; 
-    unfold run_vm_step;
-    monad_unfold;
-    eapply IHil1;
-    simpl in H;
-    unfold run_vm_step in H; simpl in *; monad_unfold; 
-    apply H).
-Admitted.
-
-Lemma double_pop : forall e e' e0 e1 st_ev st_ev0 st_stack st_stack0
-                     st_trace st_trace0 m s,
+ Lemma double_pop : forall e e' e0 e1 st_ev st_ev0 st_stack st_stack0
+                     st_trace st_trace' st_trace0 st_trace0' s,
     (Some e1,
      {| st_ev := st_ev; st_stack := st_stack; st_trace := st_trace |}) =
-    pop_stackm {| st_ev := e'; st_stack := s; st_trace := [] |} ->
+    pop_stackm {| st_ev := e'; st_stack := s; st_trace := st_trace' |} ->
     
     (Some e0,
      {| st_ev := st_ev0; st_stack := st_stack0; st_trace := st_trace0 |}) =
-    pop_stackm {| st_ev := e; st_stack := s; st_trace := m |} ->
+    pop_stackm {| st_ev := e; st_stack := s; st_trace := st_trace0' |} ->
 
     (st_stack0 = st_stack /\ e0 = e1).
 Proof.
 Admitted.
 
-(*
-Lemma pop_stackm_facts : forall e e' e0 e1 st_ev st_ev0 st_stack st_stack0
-                     st_trace st_trace0 m s,
+Lemma pop_stackm_facts : forall e' e1 st_ev st_stack
+                     st_trace st_trace' s,
     (Some e1,
      {| st_ev := st_ev; st_stack := st_stack; st_trace := st_trace |}) =
-    pop_stackm {| st_ev := e'; st_stack := s; st_trace := [] |} ->
- *)
+    pop_stackm {| st_ev := e'; st_stack := s; st_trace := st_trace' |} ->
+    (e' = st_ev /\ st_trace' = st_trace /\ (exists e, s = e::st_stack)).
+Proof.
+Admitted.
+
 
 
 Ltac do_double_pop :=
@@ -277,117 +223,6 @@ Ltac do_double_pop :=
             pop_stackm {| st_ev := ?e; st_stack := ?s; st_trace := ?m |} |- _ ] =>
     assert (st_stack0 = st_stack /\ e0 = e1) by (eapply double_pop; eauto)
   end; destruct_conjs.
-
-
-Lemma ev_irrel : forall il1 tr1 e1 e2 s s',
-(*
-    run_vm il1 {| st_ev := e; st_trace := tr1 |} =
-    {| st_ev := e'; st_trace := tr1' |} -> *)
-    
-    st_trace (
-        run_vm il1 {| st_ev := e1; st_stack := s; st_trace := tr1 |}) =
-    st_trace (
-        run_vm il1 {| st_ev := e2; st_stack := s'; st_trace := tr1 |}).
-Proof.
-  induction il1; intros.
-  - simpl.
-    reflexivity.
-  -
-      destruct a; try (
-      try destruct p; 
-    unfold run_vm_step;
-    monad_unfold;
-    try eapply IHil1;
-    simpl in *;
-    unfold run_vm_step in *; simpl in *; monad_unfold; 
-      eassumption).
-      + (* joins case *)
-        simpl.
-        unfold run_vm_step in *. monad_unfold.
-        unfold get_ev.
-        monad_unfold.
-        desp. desp.
-        pairs.
-        (*do_double_pop.*)
-        
-        assert (st_trace = st_trace0). {
-          admit. }
-        rewrite H.
-        eauto.
-        
-        destruct v; destruct v0.
-        (*
-        
-      desp.
-      desp.
-      pairs.
-      unfold pop_stackm in *. monad_unfold.
-      remember (pop_stack EvidenceC s) as p.
-      destruct p. destruct p.
-      remember (pop_stack EvidenceC s') as p.
-      destruct p. destruct p.
-      pairs.
-      eapply IHil1.
-      monad_unfold. inv Heqp0.
-      monad_unfold. inv Heqp.
-      admit.
-      desp.
-      pairs.
-      subst.
-      destruct v0.
-      destruct v.
-      pairs. subst.
-Defined. *)
-Admitted.
-
-
-
-Lemma stack_irrel : forall il1 tr1 tr1' tr2 e e' s s',
-    run_vm il1 {| st_ev := e; st_trace := tr1; st_stack := s |} =
-    {| st_ev := e'; st_trace := tr1'; st_stack := s' |} ->
-    
-    st_stack (
-        run_vm il1 {| st_ev := e; st_trace := tr2; st_stack := s |}) =
-    s'.
-  (*
-    st_trace (
-        run_vm il1 {| st_ev := e1; st_trace := tr2; st_stack := s |}).*)
-Proof.
-  induction il1; intros.
-  - simpl.
-    inversion H. reflexivity.
-  -
-    (*
-    simpl;
-    destruct a; destruct p; 
-    unfold run_vm_step;
-    monad_unfold;
-    eapply IHil1;
-    simpl in H;
-    unfold run_vm_step in H; simpl in *; monad_unfold; 
-      apply H.
-Defined. *)
-Admitted.
-
-
-Lemma hihi : forall il (m : list Ev) (e : EvidenceC) s,
-    st_trace (fold_left run_vm_step il
-                        {| st_ev := e; st_trace := m; st_stack := s |}) =
-    m ++
-      st_trace (fold_left run_vm_step il
-                          {| st_ev := e; st_trace := []; st_stack := s |}) ->
-
-    (st_trace
-       (fold_left run_vm_step il
-                  {| st_ev := e; st_trace := m; st_stack := s |})) =
-    (m ++
-       st_trace
-       (fold_left run_vm_step il
-                  {| st_ev :=  e; st_trace := []; st_stack := s |})).
-Proof.
-  intros.
-  auto.
-Defined.
 
 Lemma push_stackm_pure : forall o e st_ev st_ev0 st_stack st_stack0 st_trace st_trace0,
     (o, {| st_ev := st_ev0; st_stack := st_stack0; st_trace := st_trace0 |}) =
@@ -471,9 +306,137 @@ Proof.
   monad_unfold. inv H.
 Defined.
 
+Lemma trace_irrel : forall il1 tr1 tr1' tr2 e e' s s',
 
+    run_vm il1 {| st_ev := e; st_trace := tr1; st_stack := s |} =
+    {| st_ev := e'; st_trace := tr1'; st_stack := s' |} ->
+    
+    st_ev (
+        run_vm il1 {| st_ev := e; st_trace := tr2; st_stack := s |}) = e'.
+Proof.
+  induction il1; intros.
+  - simpl.
+    inversion H. reflexivity.
+    
+  -
+    simpl;
+    destruct a; try (destruct p; 
+    unfold run_vm_step;
+    monad_unfold;
+    eapply IHil1;
+    simpl in H;
+    unfold run_vm_step in H; simpl in *; monad_unfold; 
+    eassumption).
+Admitted.
 
+Lemma ev_irrel : forall il1 tr1 e1 e2 s s',
+(*
+    run_vm il1 {| st_ev := e; st_trace := tr1 |} =
+    {| st_ev := e'; st_trace := tr1' |} -> *)
+    
+    st_trace (
+        run_vm il1 {| st_ev := e1; st_stack := s; st_trace := tr1 |}) =
+    st_trace (
+        run_vm il1 {| st_ev := e2; st_stack := s'; st_trace := tr1 |}).
+Proof.
+  induction il1; intros.
+  - simpl.
+    reflexivity.
+  -
+      destruct a; try (
+      try destruct p; 
+    unfold run_vm_step;
+    monad_unfold;
+    try eapply IHil1;
+    simpl in *;
+    unfold run_vm_step in *; simpl in *; monad_unfold; 
+      eassumption).
+      + (* joins case *)
+        simpl.
+        unfold run_vm_step in *. monad_unfold.
+        unfold get_ev.
+        monad_unfold.
+        desp. desp.
+        pairs.
+        (*do_double_pop.*)
+        
+        assert (st_trace = st_trace0). {
+          admit. }
+        rewrite H.
+        eauto.
+        
+        destruct v; destruct v0.
+        (*
+        
+      desp.
+      desp.
+      pairs.
+      unfold pop_stackm in *. monad_unfold.
+      remember (pop_stack EvidenceC s) as p.
+      destruct p. destruct p.
+      remember (pop_stack EvidenceC s') as p.
+      destruct p. destruct p.
+      pairs.
+      eapply IHil1.
+      monad_unfold. inv Heqp0.
+      monad_unfold. inv Heqp.
+      admit.
+      desp.
+      pairs.
+      subst.
+      destruct v0.
+      destruct v.
+      pairs. subst.
+Defined. *)
+Admitted.
 
+Lemma stack_irrel : forall il1 tr1 tr1' tr2 e e' s s',
+    run_vm il1 {| st_ev := e; st_trace := tr1; st_stack := s |} =
+    {| st_ev := e'; st_trace := tr1'; st_stack := s' |} ->
+    
+    st_stack (
+        run_vm il1 {| st_ev := e; st_trace := tr2; st_stack := s |}) =
+    s'.
+  (*
+    st_trace (
+        run_vm il1 {| st_ev := e1; st_trace := tr2; st_stack := s |}).*)
+Proof.
+  induction il1; intros.
+  - simpl.
+    inversion H. reflexivity.
+  -
+    (*
+    simpl;
+    destruct a; destruct p; 
+    unfold run_vm_step;
+    monad_unfold;
+    eapply IHil1;
+    simpl in H;
+    unfold run_vm_step in H; simpl in *; monad_unfold; 
+      apply H.
+Defined. *)
+Admitted.
+
+(*
+Lemma hihi : forall il (m : list Ev) (e : EvidenceC) s,
+    st_trace (fold_left run_vm_step il
+                        {| st_ev := e; st_trace := m; st_stack := s |}) =
+    m ++
+      st_trace (fold_left run_vm_step il
+                          {| st_ev := e; st_trace := []; st_stack := s |}) ->
+
+    (st_trace
+       (fold_left run_vm_step il
+                  {| st_ev := e; st_trace := m; st_stack := s |})) =
+    (m ++
+       st_trace
+       (fold_left run_vm_step il
+                  {| st_ev :=  e; st_trace := []; st_stack := s |})).
+Proof.
+  intros.
+  auto.
+Defined.
+*)
 
 Lemma foo : forall il m e s,
     st_trace (fold_left run_vm_step il
@@ -487,133 +450,49 @@ Proof.
     
     unfold run_vm_step; fold run_vm_step; monad_unfold;
     
-      rewrite IHil at 1;
-      symmetry; 
-      rewrite IHil at 1;
-       (*
-    assert ( st_trace
-    (fold_left run_vm_step il
-               {| st_ev := prim_ev p e; st_trace := prim_trace n p; st_stack := s |}) =
-             
-             (prim_trace n p) ++
-                              st_trace (fold_left run_vm_step il
-                                                  {| st_ev := prim_ev p e; st_trace := []; st_stack := s |})) as H by (apply IHil);
-    
-    rewrite H; *)
-    
-    (*erewrite hihi; eauto; *)
+    rewrite IHil at 1;
+    symmetry; 
+    rewrite IHil at 1;
+
     rewrite <- app_assoc;
     tauto).
     
     
     + (* joins case *)
       unfold run_vm_step; fold run_vm_step; monad_unfold; monad_unfold.
-
-      
-    
-
-     desp.
-
-      
-      (*
-
-      remember (pop_stackm {| st_ev := e; st_stack := s; st_trace := m |}) as p; 
-      destruct p;
-      destruct o. *)
-
-      (*
-      remember ( push_stackm (ssc e0 e) v) as q.
-      destruct q.
-      destruct o. simpl.
-      dependent destruction v.
-      dependent destruction v0.
-      simpl. *)
-
-     desp.
-     pairs.
-
-     (*
-       remember (pop_stackm {| st_ev := e; st_stack := s; st_trace := [] |}) as r.
-      destruct r.
-      destruct o. *)
-
-      (*
-      remember (push_stackm (ssc e1 e) v) as y.
-      destruct y. destruct o. *)
-(*
-      dependent destruction v.
-      dependent destruction v0.
-      monad_unfold. *)
+      desp.
+      desp.
+      pairs.
       rewrite IHil at 1.
-      
       symmetry.
       rewrite IHil at 1.
       assert (st_trace0 = m ++ st_trace). {
         assert (st_trace0 = m). {
-          
-          
-
-
           eapply pop_stackm_pure; eauto. 
            }
         assert (st_trace = []). {
-
-
-
           eapply pop_stackm_pure; eauto.
         }
         subst.
         rewrite app_nil_r. congruence.
       }
-
-      rewrite H.
-      rewrite app_assoc at 1.
-      rewrite app_assoc at 1.
-
+      subst.
       do_double_pop.
-        (*
-      assert (e0 = e1). {
-        
-        
-        
-        }
-      assert (st_stack0 = st_stack). admit. *)
-     
-      congruence.
-      (*
-      erewrite ev_irrel.
-      reflexivity. *)
-      dependent destruction v.
-      dependent destruction v0.
-      
 
+      rewrite app_assoc at 1.
+      rewrite app_assoc at 1.
+      congruence.
+
+      destruct v;
+      destruct v0.
+  
       elimtype False; eapply pop_stackm_determ_none; eauto.
       desp.
 
       destruct v; destruct v0.
 
       elimtype False; eapply pop_stackm_determ_none; eauto.
-      
-
-
-
-      
-      
-        
-      (*elimtype False; eapply push_stackm_succeeds; eauto. *)
-
-      (*
-      remember (pop_stackm {| st_ev := e; st_stack := s; st_trace := [] |}) as r.
-      destruct r.
-      destruct o. *)
-      
-      
-      (*
-      remember (push_stackm (ssc e0 e) v0) as r.
-      destruct r.
-      destruct o. *)
-      destruct v.
-      destruct v0.
+     
       pairs.
       subst.
       rewrite IHil.
@@ -624,48 +503,22 @@ Proof.
       
 
       desp.
-      (*
-      remember (pop_stackm {| st_ev := e; st_stack := s; st_trace := m |}) as p.
-      destruct p.
-      destruct o. *)
-
       desp.
-      (*
-      remember (push_stackm e v) as q.
-      destruct q.
-      destruct o. *)
+
       
-      dependent destruction v.
-      dependent destruction v0.
+      destruct v;
+      destruct v0.
       simpl.
-
-      (*
-      remember (pop_stackm {| st_ev := e; st_stack := s; st_trace := [] |}) as r.
-      destruct r.
-      destruct o.
-
-      remember (push_stackm e v) as y.
-      destruct y.
-      destruct o.
-
-      dependent destruction v.
-      dependent destruction v0.
-       *)
       
       rewrite IHil at 1.
       symmetry.
       rewrite IHil at 1.
       assert (st_trace = m ++ st_trace0). {
         assert (m = st_trace). {
-          
-
           symmetry.
           eapply pop_stackm_pure; eauto.
            }
         assert (st_trace0 = []). {
-
-
-
           eapply pop_stackm_pure; eauto.
         }
         subst.
@@ -677,215 +530,27 @@ Proof.
 
       do_double_pop.
       congruence.
-(*
-      assert (e0 = e1). admit.
-      assert (st_stack0 = st_stack). admit.
-
-
-      congruence. *)
-
-      (*
-      erewrite ev_irrel.
-      reflexivity. *)
-      
-
-(*
-      assert (False). eapply push_stackm_succeeds; eauto. contradiction. *)
-
-
 
       destruct v; destruct v0.
       elimtype False; eapply pop_stackm_determ_none; eauto.
       desp.
-      destruct v; destruct v0.
-      
+      destruct v; destruct v0.    
       elimtype False; eapply pop_stackm_determ_none; eauto.
       destruct v; destruct v0.
       rewrite IHil.
       symmetry.
       rewrite IHil.
 
-      (*
-      eassumption.
-
-      contradiction.
-      
-        
-      assert (False). eapply push_stackm_succeeds; eauto. contradiction.
-
-      remember (pop_stackm {| st_ev := e; st_stack := s; st_trace := [] |}) as r.
-      destruct r.
-      destruct o.
-      
-      remember (push_stackm e v0) as r.
-      destruct r.
-      destruct o.
-      dependent destruction v.
-      dependent destruction v0.
-      assert (False). eapply pop_stackm_determ; eauto. contradiction.
-
-      assert (False). eapply push_stackm_succeeds; eauto. contradiction.
-      
-     
-      simpl.
-      dependent destruction v.
-      dependent destruction v0.
-      assert (s = st_stack). {
-      eapply pop_stackm_fail; eauto. }
-      subst. *)
       assert (st_trace = m /\ e = st_ev). {
-     
         eapply pop_stackm_pure; eauto. }
-
       assert (st_trace0 = [] /\ e = st_ev0). {
         eapply pop_stackm_pure; eauto. }
       destruct_conjs.
       subst.
-     
-
-      assert (st_stack = st_stack0). {
-       
+      assert (st_stack = st_stack0). {       
         eapply pop_stackm_determ_n; eauto. }
       subst. simpl. auto.
 Defined.
-
-
-(*
-Lemma multi_implies_run: forall il tr e e' s s',
-  vm_multi (mk_config e il s) (mk_config e' [] s') tr ->
-  run_vm il (mk_st e s []) = {| st_ev := e'; st_trace := tr; st_stack := s' |}.
-Proof.
-  induction il; intros.
-  - inv H; unfold run_vm; simpl.
-    + reflexivity.
-    + inv H0.
-  - inv H.
-    unfold run_vm; simpl.
-    unfold run_vm_step. fold run_vm_step. unfold execSt.
-
-    (*destruct a; destruct p; dependent destruction x'; inv H0; inv H0; simpl in *. *)
-    dependent destruction x'; inv H0; inv H0; simpl in *.
-
-    (* pose (IHil cs' (hhc (hashEv e) e) e'). simpl in *. *)
-    destruct a.
-    Check prim_ev.
-    pose (IHil cs' (prim_ev p e) e' s s'). simpl in *. 
-
-    concludes.
-    Check foo.   
-    assert    ( st_trace (fold_left run_vm_step vm_list0
-                        {| st_ev := prim_ev p e; st_trace := prim_trace n p; st_stack := s |}) =
-    prim_trace n p ++ st_trace (fold_left run_vm_step vm_list0
-                                         {| st_ev := prim_ev p e; st_trace := []; st_stack := s |})) as H2.
-    apply foo.
-    apply st_congr;
-      try (eapply trace_irrel; eassumption).
-    eapply stack_irrel; eassumption.
-    
-    rewrite H2. simpl.
-    assert ( run_vm vm_list0 {| st_ev := prim_ev p e; st_trace := []; st_stack := s |} =
-             (fold_left run_vm_step vm_list0 {| st_ev := prim_ev p e; st_trace := []; st_stack := s |})) as H3.
-    { auto. }
-    rewrite <- H3.
-    rewrite e0. simpl. auto.
-Defined.
-
-
-Lemma vm_multi_trans : forall x y z tr tr',
-  vm_multi x y tr ->
-  vm_multi y z tr' ->
-  vm_multi x z (tr ++ tr').
-Proof.
-  apply refl_trans_1n_trace_trans.
-Defined.
-
-Lemma run_implies_multi: forall il tr e e' s s',
-    run_vm il {| st_ev := e; st_trace := []; st_stack := s |} = {| st_ev := e'; st_trace := tr; st_stack := s' |} ->
-    vm_multi (mk_config e il s) (mk_config e' [] s') tr.
-Proof. 
-  induction il; intros.
-  - inv H; unfold run_vm; simpl.
-    econstructor.
-  - 
-    unfold run_vm in H.
-    assert (a :: il = [a]++il) as H0. auto.
-    rewrite H0 in *.
-    rewrite fold_left_app in H. simpl in H. unfold run_vm_step in H. fold run_vm_step in H.
-
-    
-    unfold run_vm in IHil.   
-    destruct a.
-    Check prim_trace.
-    monad_unfold.
-    unfold run_vm_step in H. fold run_vm_step in H.
-
-    assert (
-       st_trace ( fold_left run_vm_step il
-        {| st_ev := prim_ev p e; st_trace := prim_trace n p; st_stack := s |}) =
-        st_trace ({| st_ev := e'; st_trace := tr; st_stack := s' |})
-      ).
-    { congruence. }
-
-    assert (
-      st_ev (fold_left run_vm_step il
-        {| st_ev := prim_ev p e; st_trace := prim_trace n p; st_stack := s |}) =
-      st_ev ({| st_ev := e'; st_trace := tr; st_stack := s' |})).
-    { congruence. }
-
-    simpl in *.
-         
-    assert (st_trace (fold_left run_vm_step il
-                                {| st_ev := e; st_trace := prim_trace n p; st_stack := s |}) =
-            (prim_trace n p) ++ st_trace (fold_left run_vm_step il {| st_ev := e; st_trace := []; st_stack := s |})).
-    apply foo.
-
-    assert (st_trace
-         (fold_left run_vm_step il
-                    {| st_ev := e; st_trace := prim_trace n p; st_stack := s |}) =
-            st_trace
-         (fold_left run_vm_step il
-                    {| st_ev := prim_ev p e; st_trace := prim_trace n p; st_stack := s |})).
-    eapply ev_irrel.
-    rewrite <- H4 in H1.
-    rewrite H3 in H1.
-    rewrite <- H1.
-    
-    econstructor.
-    econstructor.
-    simpl.
-    eapply IHil.
-
-    apply st_congr.
-    eapply trace_irrel.
-    monad_unfold.
-
-    apply H.
-    eapply stack_irrel; eauto.
-    eapply ev_irrel.
-Defined.
-
-
-Lemma run_iff_multi: forall il tr e e' s s',
-run_vm il {| st_ev := e; st_trace := []; st_stack := s |} = {| st_ev := e'; st_trace := tr; st_stack := s' |} <->
-vm_multi (mk_config e il s) (mk_config e' [] s') tr.
-Proof.
-  intros.
-  split.
-  - apply run_implies_multi.
-  - apply multi_implies_run.
-Defined.
-*)
-
-(*
-Lemma ha : forall e e' e'' s s' s'' il1 il2 resl tr1 tr2,
-  vm_multi (mk_config e  (il1 ++ il2) s) (mk_config e' il2 s') tr1 ->
-  vm_multi (mk_config e' il2 s') (mk_config e'' resl s'') tr2  ->
-  vm_multi (mk_config e  (il1 ++ il2) s) (mk_config e'' resl s'') (tr1 ++ tr2).
-Proof.
-  intros.
-  eapply vm_multi_trans; eauto.
-Defined.
-*)
 
 (*
 Lemma asas : forall i l l' tr e e' s s',
@@ -902,44 +567,6 @@ Proof.
 Defined.
 *)
 
-Print vm_st.
-
-(*
-
-Lemma vm_multi_transitive:
-  forall il1 il2 resl tr1 tr2 e e' e'' s s' s'',
-    vm_multi (mk_config e il1 s) (mk_config e' [] s') tr1 ->
-    vm_multi (mk_config e' il2 s') (mk_config e'' resl s'') tr2 ->
-    vm_multi (mk_config e (il1 ++ il2) s) (mk_config e'' resl s'') (tr1 ++ tr2).     
-Proof.
-  intros.
-  dependent induction H.
-  - simpl. eauto.
-  - simpl.
-    rewrite <- app_assoc.
-    dependent destruction x'.
-    inv H.
-    monad_unfold.
-    (*assert ((i :: vm_list0) ++ il2 = (i::(vm_list0 ++ il2))). auto.
-    rewrite H2.*)
-    constructor 2 with (x':=(mk_config (st_ev res_st) (vm_list0 ++ il2) (st_stack res_st))).
-    eapply asas.
-    eassumption.
-    eapply IHrefl_trans_1n_trace; eauto.
-Defined.
- *)
-
-Check vm_st.
-Print vm_st.
-Print run_vm.
-(*
-{ st_ev : EvidenceC;  st_stack : ev_stack;  st_trace : list Ev }
-
-run_vm = 
-fun (il : list AnnoInstr) (st : vm_st) => fold_left run_vm_step il st
-     : list AnnoInstr -> vm_st -> vm_st
-*)
-
 (*
 Lemma run_transitive_done: forall il1 il2 tr1 tr2 e e' e'' s s' s'',
     run_vm il1 (mk_st e s []) = (mk_st e' s' tr1) ->
@@ -949,75 +576,7 @@ Proof.
 Admitted.
 *)
 
-(*
-Lemma vm_multi_transitive_done: forall il1 il2 tr1 tr2 e e' e'' s s' s'',
-    vm_multi (mk_config e il1 s) (mk_config e' [] s') tr1 ->
-    vm_multi (mk_config e' il2 s') (mk_config e'' [] s'') tr2 ->
-    vm_multi (mk_config e (il1 ++ il2) s) (mk_config e'' [] s'') (tr1 ++ tr2).
-Proof.
-  intros.
-  eapply vm_multi_transitive; eauto.
-Defined. 
-*)
 
-(*
-Definition vm_n1_multi : step_relation vm_config Ev := refl_trans_n1_trace vm_step.
-
-Lemma vm_n1_implies_1n : forall r r' tr,
-    vm_n1_multi r r' tr -> vm_multi r r' tr.
-Proof.
-  intros.
-  apply refl_trans_n1_1n_trace; eauto.
-Defined.
-
-Lemma vm_1n_implies_n1 : forall r r' tr,
-    vm_multi r r' tr -> vm_n1_multi r r' tr.
-Proof.
-  intros.
-  apply refl_trans_1n_n1_trace; eauto.
-Defined.
-
-Lemma vm_1n_iff_n1 : forall r r' tr,
-    vm_multi r r' tr <-> vm_n1_multi r r' tr.
-Proof.
-  intros.
-  split.
-  - apply vm_1n_implies_n1.
-  - apply vm_n1_implies_1n.
-Defined.
-*)
-
-(*
-Lemma vm_n1_multi_transitive:
-  forall e e' e'' s s' s'' il1 il2 resl tr1 tr2,
-    vm_n1_multi (mk_config e il1 s) (mk_config e' [] s') tr1 ->
-    vm_n1_multi (mk_config e' il2 s') (mk_config e'' resl s'') tr2 ->
-    vm_n1_multi (mk_config e (il1 ++ il2) s) (mk_config e'' resl s'') (tr1 ++ tr2).
-Proof.
-  intros.
-  rewrite <- vm_1n_iff_n1 in *.
-  eapply vm_multi_transitive; eauto.
-Defined.
-*)
-
-(* 
-Record vm_config : Type :=
-  mk_config
-    {vm_ev:EvidenceC ; 
-      vm_stack:ev_stack ;
-     vm_list:list AnnoInstr}.
- *)
-(*
-Lemma record_congr : forall r,
-  r = 
-  {| vm_ev := vm_ev r; vm_list := vm_list r; vm_stack := vm_stack r |}.
-Proof.
-  intros.
-  destruct r.
-  reflexivity.
-Defined.
- *)
-Check st_congr.
 
 (*
 Lemma restt : forall tr1 tr2 il il1 i e e' e'' s s' s'',
@@ -1092,150 +651,6 @@ Proof.
   simpl. rewrite <- app_assoc. eauto.
 Defined.
 
-(*
-Theorem vm_multi_suffix : forall il1 il2 tr e e' s s',
-    vm_multi {| vm_ev := e; vm_list := il1; vm_stack := s |} {| vm_ev := e'; vm_list := il2; vm_stack := s' |} tr ->
-    exists prefix, il1 = prefix ++ il2.
-Proof.
-  dependent induction il1; destruct il2; intros.
-  - exists []. reflexivity.
-  - inv H. inv H0.
-  - exists (a::il1). rewrite app_nil_r. reflexivity.
-  - inv H.
-    + exists []. reflexivity.
-    + dependent destruction x'.
-      assert (vm_list0 = il1).
-      inv H0. reflexivity.   
-      edestruct IHil1.
-      rewrite H2 in H1.
-      apply H1.
-      rewrite H3.
-      exists (a::x). reflexivity.
-Defined.
-*)
-
-(*
-Lemma il1_pieces' : forall i0 vm_list0 il1 il2 i tr e e' s s',
-    i0 :: vm_list0 = il1 ++ il2 ->
-    vm_multi {| vm_ev := e; vm_list := vm_list0; vm_stack := s |} {| vm_ev := e'; vm_list := i :: il2; vm_stack := s' |} tr ->
-    exists bla, il1 = [i0] ++ bla ++ [i].
-Proof.
-  intros i0 vm_list0 il1 il2 i tr e e' s s' H0 H1.
-  remember (vm_multi_suffix _ _ _ _ _ _ _ H1) as e2. destruct e2. exists x.
-  apply headShouldersKneesAndToes with (t := vm_list0) (l2 := il2); try assumption.
-Qed.
-*)
-
-(*
-Lemma restl : forall i il1 il2 cs cs' e e' e'' s s' s'',
-  vm_multi  (mk_config e (il1 ++ il2) s) (mk_config e' (i::il2) s') cs ->
-  vm_step (mk_config e' [i] s') (mk_config e'' [] s'') cs' ->
-  vm_multi  (mk_config e il1 s) (mk_config e'' [] s'') (cs ++ cs').
-Proof.
-  intros.
-  dependent induction H.
-  - assert (il1 = [i]).
-    eapply listThing; eauto.
-    rewrite H in *. clear x. clear H.
-    eapply step_implies_multi; eauto.
-  - dependent destruction x'.
-    inv H.
-    monad_unfold.
-    rewrite <- app_assoc.
-
-    assert (exists bla, il1 = [i0] ++ bla ++ [i]).
-    eapply il1_pieces'; eauto.
-    destruct_conjs.
-    rewrite H3.
-    rewrite H3 in H.
-
-    assert (
-        (H2 ++ [i] ++ il2) =
-        vm_list0).
-      {
-        assert (i0::vm_list0 = [i0]++vm_list0).
-        { auto. }
-        rewrite H3 in H4.
-
-        rewrite <- app_assoc in H4.
-        assert (([i0] ++ (H2 ++ [i]) ++ il2) =
-                i0 :: (H2 ++ [i] ++ il2)).
-        {
-          rewrite <- app_assoc.
-          simpl. auto.
-        }
-
-        rewrite H6 in H4.
-        congruence.
-      } 
-    rewrite <- H5 in H.
-
-    Check asas.
-    assert (([i0] ++ H2 ++ [i]) ++ il2  = i0 :: (H2 ++ [i] ++ il2)).
-    {
-      simpl.
-      rewrite <- app_assoc.
-      assert ([i]++il2 = i::il2). auto.
-      rewrite H6. auto.
-    }
-    rewrite H6 in H.
-    
-    eapply vm_multi_transitive.
-    eapply step_implies_multi.
-    Check asas.
-
-    eapply asas. apply H.
-    eapply IHrefl_trans_1n_trace; eauto.
-    rewrite <- app_assoc.
-    subst. auto.
-Defined.
-*)
-
-(*
-Lemma restl' : forall il1 il2 tr e e' s s',
-    vm_multi  (mk_config e (il1 ++ il2) s)
-                 (mk_config e' il2 s') tr ->
-    vm_multi  (mk_config e il1 s) (mk_config e' [] s') tr.
-Proof.
-  intros.
-  inv H.
-  - assert (il1 = []).
-    { eapply hh; eauto. }
-    subst.    
-    econstructor.
-  - rewrite vm_1n_iff_n1 in H.
-    inv H.
-    + assert (il1 = []).
-      eapply hh; eauto.
-      subst.
-      econstructor.
-    + dependent destruction x'0.
-      assert (exists i, vm_list0 = i :: il2).
-      dependent destruction vm_list0. inv H6. inv H6.
-      dependent destruction x'.
-      exists a. reflexivity.
-
-      destruct_conjs.
-      rewrite H5 in *.
-      eapply restl.
-      rewrite vm_1n_iff_n1. apply H3.
-      eapply asas. eauto.
-Defined.
-*)
-
-(*
-Lemma fafa : forall tr i rest e e' s s',
-    vm_step (mk_config e [i] s) (mk_config e' [] s') tr ->
-    vm_multi (mk_config e ([i] ++ rest) s) (mk_config e' rest s') tr.
-Proof.
-  intros.
-  assert (tr = tr ++ []). rewrite app_nil_r. auto. rewrite H0.
-  econstructor.
-  eapply asas. eauto.
-  econstructor.
-Defined.
-*)
-
 Lemma list_nil_app{A:Type} : forall (l1 l2:list A),
     [] = l1 ++ l2 ->
     l1 = [] /\ l2 = [].
@@ -1292,7 +707,7 @@ Proof.
 Defined.
 *)
 
-(*
+
 Lemma put_ev_after_immut_stack{A:Type} : forall s (h:VM A) e,
     st_stack (execSt s h) = st_stack (execSt s (h ;; (put_ev e))).
 Proof.
@@ -1305,7 +720,6 @@ Proof.
   destruct (h {| st_ev := st_ev; st_stack := st_stack; st_trace := st_trace |}).
   destruct o; eauto.
 Defined.
-*)
 
 (*
 Lemma update_ev_immut_stack'{A:Type} : forall s (h:VM A) e,
@@ -1314,15 +728,6 @@ Proof.
 Abort.
 *)  (* NOT true for arbitrary h:  h could match on e to update its stack *)
 
-
-(*
-Ltac invv :=
-  repeat (
-      match goal with
-      | [ H: vm_lstar _ _ (_::_) _ _ |- _ ] => inv H; doit
-      | [ G: vm_step _ _ _ _ |- _ ] => inv G; doit
-      end).
-*)
 
 Lemma ssc_inv : forall e1 e1' e2 e2',
     e1 = e1' ->
@@ -1336,619 +741,8 @@ Defined.
 Axiom para_eval_vm : forall t e,
     parallel_eval_thread (unanno t) e = parallel_att_vm_thread (instr_compiler t) e.
 
-(*
-Lemma jj_gen : forall il1 rest tr e e' s s',
-    vm_multi
-      {| vm_ev := e; vm_list := il1; vm_stack := s |}
-      {| vm_ev := e'; vm_list := []; vm_stack := s' |} tr ->
-    
-    vm_multi
-      {| vm_ev := e;
-         vm_list := il1 ++ rest; vm_stack := s
-          |}
-      {| vm_ev := e';
-         vm_list := rest; vm_stack := s'
-          |} tr.
-Proof.
-  intros il1 rest tr e e' s s' H.
-  assert (rest = [] ++ rest). simpl. reflexivity.
-  rewrite H0 at 2.
-  assert (tr = tr ++ []). rewrite app_nil_r. auto.
-  rewrite H1.
-  eapply vm_multi_transitive. apply H.
-  simpl. econstructor.
-Defined.
-*)
-
-(*
-Lemma ev_determ : forall il e s tr1 tr1' e' s' tr2,
-    fold_left run_vm_step il {| st_ev := e; st_stack := s; st_trace := tr1 |} =
-    {| st_ev := e'; st_stack := s'; st_trace := tr1' |} ->
-    st_ev (fold_left run_vm_step il {| st_ev := e; st_stack := s; st_trace := tr2 |}) = e'.
-Proof.
-  induction il; intros.
-  - simpl. simpl in H. congruence.
-  - simpl;
-    unfold run_vm_step; fold run_vm_step;
-    destruct a; try (simpl; monad_unfold;
-    try (destruct p); simpl;
-    eapply IHil; simpl in *; unfold run_vm_step in *; fold run_vm_step in H; simpl in *;
-    unfold execSt in *; simpl in *; eassumption).
-    + (* joins case *)
-      
-      unfold run_vm_step in *. fold run_vm_step in *. monad_unfold.
-      unfold run_vm_step in H. fold run_vm_step in H. monad_unfold.
-      unfold get_ev in *. monad_unfold.
-      
-
-      remember (pop_stackm {| st_ev := e; st_stack := s; st_trace := tr2 |}) as r.
-      destruct r. destruct o.
-(*
-      remember (push_stackm (ssc e0 e) v) as p.
-      destruct p. destruct o. *)
-      simpl.
-      
-      remember (pop_stackm {| st_ev := e; st_stack := s; st_trace := tr1 |}) as r.
-      destruct r. destruct o.
-(*
-      remember (push_stackm (ssc e1 e) v1) as p.
-      destruct p. destruct o. *)
-      simpl in *. monad_unfold.
-      unfold add_trace in *.
-      dependent destruction v.
-      (*dependent destruction v2.*)
-      dependent destruction v0.
-      (*dependent destruction v1. *)
-      eapply IHil.
-      assert (st_ev2 = st_ev0). {
-        assert (st_ev = st_ev0). {
-          admit. }
-        rewrite <- H0. clear Heqp0.
-        assert (st_ev1 = st_ev2). {
-          admit. }
-        rewrite <- H1.
-        assert (e = st_ev1). {
-          admit. }
-        rewrite <- H2.
-        eapply pop_stackm_pure; eauto. }
-      
-      subst.
-
-      assert (st_stack2 = st_stack0). {
-        admit. (* push/pops correspond on s *)
-      }
-      subst. eassumption.
-          
-        
-        
-      admit.
-
-
-      dependent destruction v.
-      dependent destruction v0.
-      admit.
-      admit.
-      
-
-      remember (pop_stackm {| st_ev := e; st_stack := s; st_trace := tr1 |}) as r.
-      destruct r. destruct o.
-
-      remember (push_stackm (ssc e0 e) v0) as p.
-      destruct p. destruct o.
-      dependent destruction v.
-      dependent destruction v0.
-      dependent destruction v1.
-      simpl in *.
-      admit.
-      admit.
-      simpl in *.
-      dependent destruction v.
-      dependent destruction v0.
-
-      eapply IHil.
-      assert (st_ev0 = st_ev). {
-        admit. }
-      assert (st_stack0 = st_stack). {
-        admit. }
-      subst. eassumption.
-    + (* besr case *)
-Admitted.
-*)
-
-(*
-Lemma stack_determ : forall il e s tr1 tr1' e' s' tr1'',
-    fold_left run_vm_step il {| st_ev := e; st_stack := s; st_trace := tr1 |} =
-    {| st_ev := e'; st_stack := s'; st_trace := tr1' |} ->
-    st_stack (fold_left run_vm_step il {| st_ev := e; st_stack := s; st_trace := tr1'' |}) = s'.
-Proof.
-  (*
-    induction il; intros.
-  - simpl. simpl in H. congruence.
-  - simpl;
-    unfold run_vm_step; fold run_vm_step;
-    destruct a; simpl; monad_unfold;
-    destruct p; simpl;
-    eapply IHil; simpl in *; unfold run_vm_step in *; fold run_vm_step in H; simpl in *;
-      unfold execSt in *; simpl in *; eassumption.
-
-Defined. *)
-Admitted.
-*)
-
-   (*   
-Lemma run_vm_monotonic' : forall il x x0 e s,
-    st_trace (fold_left run_vm_step il
-                        {| st_ev := e; st_trace := []; st_stack := s |}) = x0 ->
-    st_trace (fold_left run_vm_step il
-                        {| st_ev := e; st_trace := x; st_stack := s |}) = x ++ x0.
-Proof.
-  intros.
-  rewrite foo in H. simpl in H. subst.
-  rewrite foo. auto.
-Defined.
-    
-Lemma run_vm_monotonic : forall il x x0 e e' s s',
-    fold_left run_vm_step il
-              {| st_ev := e; st_trace := []; st_stack := s |} =
-    {| st_ev := e'; st_trace := x0; st_stack := s' |} ->
-    fold_left run_vm_step il
-              {| st_ev := e; st_trace := x; st_stack := s |} =
-    {| st_ev := e'; st_trace := x ++ x0; st_stack := s' |}.
-Proof.
-  intros.
-  assert (st_trace (fold_left run_vm_step il {| st_ev :=e; st_trace := x; st_stack := s |}) = x ++ x0).
-  { 
-    apply run_vm_monotonic'.
-    assert (fold_left run_vm_step il {| st_ev := e; st_trace := []; st_stack := s |} =
-            {| st_ev := e'; st_trace := x0; st_stack := s' |} ->
-            st_trace (fold_left run_vm_step il {| st_ev := e; st_trace := []; st_stack := s |}) =
-            st_trace ({| st_ev := e'; st_trace := x0; st_stack := s' |})).
-    { congruence. }
-    
-  apply H0 in H.
-  simpl in H. auto. }
-       (*      
-  assert (st_ev (fold_left run_vm_step il {| st_trace := x |}) = e').
-  eapply ev_determ. eassumption. (* TODO: ev deterministic regardless of trace, stack *)
-  assert (st_stack (fold_left run_vm_step il {| st_trace := x |}) = s).
-  eapply stack_determ. eassumption. (* TODO stack deterministic regardless of trace, ev *)
-*)
-
-  apply st_congr; eauto.
-  eapply trace_irrel; eauto.
-  eapply stack_irrel; eauto.
-Defined.
-*)
-
 Ltac heee l :=
   assert (l = l ++ []) as HH; auto; rewrite HH.
-
-(*
-Ltac hee :=
-      match goal with
-      | |- context
-              [  vm_multi
-                   {| vm_ev := _; vm_list := ?x |}
-                   {| vm_ev := _; vm_list := [] |} _
-        ] =>  assert (x = x ++ []) as HH; auto; rewrite HH
-      end.
-*)
-(*
-Lemma exists_trace : forall t e s,
-  exists tr,
-  run_vm (instr_compiler t) (mk_st e s []) =
-              (mk_st (eval (unanno t) e) s tr).
-Proof.
-  induction t; intros.
-  -
-    (*exists (prim_trace (fst r) (asp_instr a)).*)
-    destruct a; 
-      simpl in *;
-      eexists; econstructor.
-  - destruct (IHt1 e s).
-    destruct (IHt2 (eval (unanno t1) e) s).
-    eexists.
-    simpl.
-    eapply run_transitive_done.
-    eassumption.
-    eassumption.
-Defined.
-*)
-
-  (*
-Lemma exists_trace : forall t e s,
-  exists tr,
-  vm_multi (mk_config e (instr_compiler t) s)
-              (mk_config (eval (unanno t) e) [] s) tr.
-Proof.
-  induction t; intros.
-  -
-    (*exists (prim_trace (fst r) (asp_instr a)).*)
-    destruct a; 
-      simpl in *;
-      eexists;
-    hee;
-    repeat econstructor.
-  - destruct (IHt1 e s).
-    destruct (IHt2 (eval (unanno t1) e) s).
-    eexists.
-    simpl.
-    eapply vm_multi_transitive_done.
-    eassumption.
-    eassumption.
-Defined.
-*)
-
-(*
-Lemma exists_trace_gen : forall il e,
-  exists tr e',
-  vm_multi (mk_config e il)
-              (mk_config e' []) tr.
-Proof.
-  induction il; intros.
-  - eexists.
-    eexists.
-    econstructor.
-  - edestruct IHil.
-    destruct_conjs.
-    destruct a.
-    destruct p.
-    eexists. exists H.
-    econstructor.
-    econstructor.
-    apply H0.
-Defined.
-
-(*
-    destruct IHt1.
-    destruct IHt2.
-    destruct_conjs.
-    exists (x ++ x0).
-    repeat eexists.
-
-    rewrite <- run_iff_multi.
-    unfold run_vm. simpl.
-    rewrite fold_left_app.
-
-    subst.
-    assert ({| st_trace := x |} =
-
-        (fold_left run_vm_step (instr_compiler t1)
-                       {| st_trace := [] |})
-            ).
-    {
-      Check run_iff_multi.
-      
-      subst.
-      rewrite <- run_iff_multi in H. unfold run_vm in H.
-     
-      congruence.
-    }
-    rewrite <- H1.
-    Check run_iff_multi.
-    
-    rewrite <- run_iff_multi in H0. unfold run_vm in H0.
-
-    apply run_vm_monotonic; eauto.
-Defined.
-*)
-*)
-
-
-(*
-Lemma trace_unique : forall il tr1 tr2 e e' e'' s s',
-    vm_multi {| vm_ev := e; vm_list := il; vm_stack := s |} {| vm_ev := e'; vm_list := []; vm_stack := s' |} tr1 ->
-    vm_multi {| vm_ev := e; vm_list := il; vm_stack := s|} {| vm_ev := e''; vm_list := []; vm_stack := s' |} tr2 ->
-    tr1 = tr2.
-Proof.
-  intros.
-  Check run_iff_multi.
-  rewrite <- run_iff_multi in *.
-  simpl in *.
-  rewrite H in H0. congruence.
-Defined.
-
-Lemma ev_unique : forall il tr1 tr2 e e' e'' s s',
-    vm_multi {| vm_ev := e; vm_list := il; vm_stack := s |} {| vm_ev := e'; vm_list := []; vm_stack := s' |} tr1 ->
-    vm_multi {| vm_ev := e; vm_list := il; vm_stack := s |} {| vm_ev := e''; vm_list := []; vm_stack := s' |} tr2 ->
-    e' = e''.
-Proof.
-  intros.
-  Check run_iff_multi.
-  rewrite <- run_iff_multi in *.
-  simpl in *.
-  rewrite H in H0. congruence.
-Defined.
-*)
-
-(*
-Lemma trace_decompose' :  forall t1 t2 tr e e'',
-      vm_multi
-      {| vm_ev := e; vm_list := (instr_compiler t1 ++ instr_compiler t2) |}
-      {| vm_ev := e''; vm_list := []; |} tr ->
-      exists tr1,
-        vm_multi
-      {| vm_ev := e; vm_list := (instr_compiler t1 ++ instr_compiler t2) |}
-      {| vm_ev := (eval (unanno t1) e); vm_list := instr_compiler t2 |} tr1 /\
-        exists tr2,
-          vm_multi
-            {| vm_ev := (eval (unanno t1) e); vm_list := instr_compiler t2 |}
-            {| vm_ev := e''; vm_list := [] |} tr2 /\
-          tr = tr1 ++ tr2.
-Proof. *)
-
-
-(*
-Lemma trace_decompose' :  forall t1 t2 tr e e'' s s'',
-      vm_multi
-      {| vm_ev := e; vm_list := (instr_compiler t1 ++ instr_compiler t2); vm_stack := s |}
-      {| vm_ev := e''; vm_list := []; vm_stack := s'' |} tr ->
-      exists tr1 e' s',
-        vm_multi
-      {| vm_ev := e; vm_list := (instr_compiler t1 ++ instr_compiler t2); vm_stack := s |}
-      {| vm_ev := e'; vm_list := instr_compiler t2; vm_stack := s' |} tr1 /\
-        exists tr2,
-          vm_multi
-            {| vm_ev := (eval (unanno t1) e); vm_list := instr_compiler t2; vm_stack := s' |}
-            {| vm_ev := e''; vm_list := []; vm_stack := s'' |} tr2 /\
-          tr = tr1 ++ tr2.
-Proof.
-  Check exists_trace.
-  Check trace_unique.
-  intros.
-  edestruct exists_trace with (t := t1) (s:=s).
-  destruct_conjs.
-  exists x. eexists. exists s.
-  split.
-  Check jj_gen.
-  eapply jj_gen.
-  eauto.
-  destruct exists_trace with (t:=t2) (e:=eval (unanno t1) e) (s:=s).
-  destruct_conjs.
-  exists x0.
- (* assert (H0 = eval (unanno t1) e).
-  eapply multi_ev_eval; eauto.
-  assert (H2 = eval (unanno t2) H0).
-  eapply multi_ev_eval; eauto. *)
-
-    assert (instr_compiler t1 ++ instr_compiler t2 = instr_compiler (alseq (0,0) t1 t2)).
-  auto.
-  rewrite H2 in H.
-  assert (e'' = eval (unanno (alseq (0, 0) t1 t2)) e).
-  {
-    destruct exists_trace with (t:=(alseq (0, 0) t1 t2)) (e:=e) (s:=s).
-    Check ev_unique.
-    eapply ev_unique with (e:=e) (e':=e'') (e'':=eval(unanno (alseq (0,0) t1 t2)) e). apply H.
-    Check stack_irrel.
-    rewrite <- run_iff_multi.
-    Check stack_irrel.
-    eapply st_congr.
-    rewrite <- run_iff_multi in H3.
-    rewrite H3. simpl. auto.
-    eapply stack_irrel.
-    rewrite <- run_iff_multi in H.
-    apply H.
-    Check ev_irrel.
-    eapply ev_irrel. }
-  
-  (*
-  eapply multi_ev_eval; eauto.*)
-  assert (s'' = s) as H4. {
-  rewrite <- run_iff_multi in *.
-  assert (
-      st_stack (run_vm (instr_compiler (alseq (0, 0) t1 t2))
-        {| st_ev := e; st_stack := s; st_trace := [] |}) =
-      st_stack ({| st_ev := e''; st_stack := s''; st_trace := tr |})).
-  { congruence. }
-  simpl in H4.
-  destruct exists_trace with (t:=(alseq (0, 0) t1 t2)) (e:=e) (s:=s).
-  rewrite <- run_iff_multi in H5.
-  erewrite stack_irrel with (s' := s) in H4; eauto. }
-
-  split; simpl in *; subst.
-  -
-    eassumption.
-    (*
-    Check st_congr.
-    Check stack_irrel.
-    rewrite <- run_iff_multi in H1.
-    rewrite <- run_iff_multi.
-    eapply st_congr.
-    eapply trace_irrel; eauto.
-    
-    assert ( st_stack (
-                 {| st_ev := eval (unanno t1) e; st_stack := s; st_trace := [] |}) = s)
-    eapply st_congr.
-    
-    auto. *)
-  -
-    
-    assert (vm_multi
-              {| vm_ev := e; vm_list := (instr_compiler t1 ++ instr_compiler t2); vm_stack := s |}
-              {| vm_ev := eval (unanno t2) (eval (unanno t1) e); vm_list := []; vm_stack := s |} (x ++ x0)). {
-  eapply traces_append_gen.
-  eassumption.
-  eassumption. }
-
-    eapply trace_unique; eauto.
-    Unshelve. exact mtc.
-Defined.
-*)
-
-(*
-Lemma trace_decompose'_gen :  forall tr il1 il2 e e'',
-      vm_multi
-      {| vm_ev := e; vm_list := (il1 ++ il2) |}
-      {| vm_ev := e''; vm_list := []; |} tr ->
-      exists tr1 e',
-        vm_multi
-      {| vm_ev := e; vm_list := (il1 ++ il2) |}
-      {| vm_ev := e'; vm_list := il2 |} tr1 /\
-        exists tr2,
-          vm_multi
-            {| vm_ev := e'; vm_list := il2 |}
-            {| vm_ev := e''; vm_list := [] |} tr2 /\
-          tr = tr1 ++ tr2.
-Proof.
-  intros.
-  edestruct exists_trace_gen with (il:=il1).
-  destruct_conjs.
-  exists x. exists H0.
-  split.
-  Check jj_gen.
-  eapply jj_gen.
-  eauto.
-  destruct exists_trace_gen with (il:=il2) (e:=H0).
-  destruct_conjs.
-  exists x0.
-  split.
-  subst.
-  (*
-  assumption.
-
-  assert (vm_multi {| vm_list := il1 ++ il2 |}
-                   {| vm_list := [] |} (x ++ x0)).
-  apply traces_append_gen; auto.
-  eapply trace_unique; eauto.
-Defined. *)
-Admitted.
-
-*)
-
-
-(*
-Lemma trace_decompose :
-  forall tr1 tr2 tr t1 t2 e e' e'' s,
-    vm_multi
-      {| vm_ev := e;  vm_list := instr_compiler t1; vm_stack := s |}
-      {| vm_ev := e'; vm_list := []; vm_stack := s |} tr1 ->
-    vm_multi
-      {| vm_ev := e';  vm_list := instr_compiler t2; vm_stack := s |}
-      {| vm_ev := e''; vm_list := []; vm_stack := s |} tr2 ->
-    vm_multi
-      {| vm_ev := e; vm_list := (instr_compiler t1 ++ instr_compiler t2); vm_stack := s |}
-      {| vm_ev := e''; vm_list := []; vm_stack := s |} tr ->
-    tr = tr1 ++ tr2.
-Proof.
-  intros.
-  edestruct trace_decompose'. eassumption.
-  destruct_conjs.
-  subst.
-  assert (e' = eval (unanno t1) e).
-  {
-    destruct exists_trace with (t:=t1) (e:=e) (s:=s).
-    Check ev_unique.
-    eapply ev_unique; eauto.
-  }
-  subst.
-  assert (H3 = s) as H7.
-  {
-    destruct exists_trace with (t:=t1(*(alseq (0,0) t1 t2)*)) (e:=e) (s:=s).
-    
-    Check stack_irrel.
-
-    Check restl'.
-    assert (
-        vm_multi
-         {|
-         vm_ev := e;
-         vm_list := instr_compiler t1;
-         vm_stack := s |}
-         {| vm_ev := H2; vm_list := []; vm_stack := H3 |} x).
-    eapply restl'; eauto.
-
-    rewrite <- run_iff_multi in *.
-(*
-    assert (
-         st_stack (run_vm (instr_compiler t1)
-         {| st_ev := e; st_stack := s; st_trace := [] |}) =
-         st_stack ({| st_ev := H2; st_stack := H3; st_trace := x |})).
-    { congruence. } *)
-
-    assert (
-    st_stack (run_vm (instr_compiler t1)
-         {| st_ev := e; st_stack := s; st_trace := [] |}) =
-    st_stack ( {| st_ev := eval (unanno t1) e; st_stack := s; st_trace := x0 |})).
-    { congruence. }
-    simpl in H9.
-    rewrite H7 in H8. inv H8.
-    reflexivity. } 
-
-    (*
-    simpl in H9.
-                                                                       
-        
-    assert 
-
-        
-    { congruence. }
-    
-    simpl in H8. rewrite <- H8.
-    Check stack_irrel.
-    symmetry.
-    
-    eapply stack_irrel; eauto.
-    rewrite <- H6 in H8.
-    simpl in H8. rewrite <- H8 in H6. simpl in H6.
-    congruence.
-    
-    admit.
-  } *)
-  assert (tr2 = H5). {
-  Check trace_unique.
-
-                   subst.
-  eapply trace_unique; eauto.
-  }
-  subst.
-  Check restl'.
-
-  assert (vm_multi {| vm_ev := e; vm_list := instr_compiler t1; vm_stack := s |} {| vm_ev := H2; vm_list := []; vm_stack := s |} x). {
-    apply restl' with (il2:=instr_compiler t2).
-   
-    eauto. }
-  
-  assert (x = tr1).
-  eapply trace_unique; eauto.
-  congruence.
-Defined.
-*)
-
-(*
-Lemma trace_decompose_gen :
-  forall tr1 tr2 tr il1 il2 e e' e'',
-    vm_multi
-      {| vm_ev := e;  vm_list := il1 |}
-      {| vm_ev := e'; vm_list := [] |} tr1 ->
-    vm_multi
-      {| vm_ev := e';  vm_list := il2 |}
-      {| vm_ev := e''; vm_list := [] |} tr2 ->
-    vm_multi
-      {| vm_ev := e; vm_list := (il1 ++ il2) |}
-      {| vm_ev := e''; vm_list := [] |} tr ->
-    tr = tr1 ++ tr2.
-Proof.
-  (*
-  intros.
-  edestruct trace_decompose'_gen. eassumption.
-  destruct_conjs.
-  rewrite H5.
-  assert (x = tr1).
-  Check hh.
-  assert (vm_multi {| vm_list := il1 |} {| vm_list := [] |} x).
-  eapply restl'; eauto.
-
-  eapply trace_unique; eauto.
-
-  assert (H3 = tr2).
-  eapply trace_unique; eauto.
-  
-  congruence.
-Defined. *)
-Admitted.
- *)
-
-Print vm_st.
 
 Lemma ya :
   forall A,
@@ -1996,7 +790,41 @@ Proof.
   pairs. subst.
   Print pop_stack_facts.
 Admitted.
-*)
+ *)
+
+      Lemma pop_stackm_facts_none :
+        forall (e' st_ev : EvidenceC) (st_stack : ev_stack)
+         (st_trace st_trace' : list Ev) (s : ev_stack),
+       (None,
+       {| st_ev := st_ev; st_stack := st_stack; st_trace := st_trace |}) =
+       pop_stackm {| st_ev := e'; st_stack := s; st_trace := st_trace' |} ->
+       e' = st_ev /\
+       st_trace' = st_trace.
+      Proof.
+      Admitted.
+
+      Lemma push_stackm_facts : forall st_ev st_ev0 (st_trace:list Ev) (st_trace0:list Ev)
+                            st_stack st_stack0 st_trace st_trace0 H0 u,
+    (Some u, {| st_ev := st_ev0; st_stack := st_stack0; st_trace := st_trace0 |}) =
+    push_stackm H0 {| st_ev := st_ev; st_stack := st_stack; st_trace := st_trace |} ->
+    st_ev = st_ev0 /\ st_trace = st_trace0 /\ st_stack0 = H0 :: st_stack.
+Proof.
+Admitted.
+
+      Lemma double_pop_none :
+      forall (e e' st_ev st_ev0 : EvidenceC)
+         (st_stack st_stack0 : ev_stack)
+         (st_trace st_trace' st_trace0 st_trace0' : list Ev) 
+         (s : ev_stack),
+       (None,
+       {| st_ev := st_ev; st_stack := st_stack; st_trace := st_trace |}) =
+       pop_stackm {| st_ev := e'; st_stack := s; st_trace := st_trace' |} ->
+       (None,
+       {| st_ev := st_ev0; st_stack := st_stack0; st_trace := st_trace0 |}) =
+       pop_stackm {| st_ev := e; st_stack := s; st_trace := st_trace0' |} ->
+       st_stack0 = st_stack.
+      Proof.
+      Admitted.
 
 Lemma st_trace_destruct' :
   forall il1 il2 e s m,
@@ -2121,11 +949,101 @@ Proof.
       auto.
      
     + (* joins case *)
+      
+
+      
       unfold run_vm_step. fold run_vm_step.
       monad_unfold.
+      unfold get_ev. monad_unfold.
+      desp.
+      desp.
       rewrite foo.
+      pairs.
       simpl.
       rewrite IHil1.
+      edestruct (pop_stackm_facts). apply Heqp.
+      edestruct (pop_stackm_facts). apply Heqp0.
+      destruct_conjs.
+      subst.
+      simpl in *.
+      Check double_pop.
+      edestruct double_pop.
+      apply Heqp.
+      apply Heqp0.
+      subst.
+      assert (
+          {|
+       st_ev := MonadVM.st_ev
+                  (fold_left run_vm_step il1
+                     {|
+                     st_ev := ssc e0 st_ev;
+                     st_stack := st_stack0;
+                     st_trace := [] |});
+       st_stack := st_stack
+                     (fold_left run_vm_step il1
+                        {|
+                        st_ev := ssc e0 st_ev;
+                        st_stack := st_stack0;
+                        st_trace := [] |});
+       st_trace := [] |} =
+
+          {|
+          st_ev := MonadVM.st_ev
+                     (fold_left run_vm_step il1
+                        {|
+                        st_ev := ssc e0 st_ev;
+                        st_stack := st_stack0;
+                        st_trace := [join n] |});
+          st_stack := st_stack
+                        (fold_left run_vm_step il1
+                           {|
+                           st_ev := ssc e0 st_ev;
+                           st_stack := st_stack0;
+                           st_trace := [join n] |});
+          st_trace := [] |}). {
+        admit. }
+      rewrite H.
+
+      admit. (* list thing *)
+
+      Check pop_stackm_determ_none.
+
+      destruct v; destruct v0.
+      elimtype False; eapply pop_stackm_determ_none; eauto.
+
+      desp.
+      
+      destruct v; destruct v0.
+      elimtype False; eapply pop_stackm_determ_none; eauto.
+
+      Check pop_stackm_facts.
+      
+
+
+
+      destruct v; destruct v0.
+
+      edestruct pop_stackm_facts_none.
+      apply Heqp.
+      edestruct pop_stackm_facts_none.
+      apply Heqp0.
+      subst.
+      rewrite IHil1.
+      assert (st_stack = st_stack0). {
+      Check double_pop.
+      
+      eapply double_pop_none; eauto. }
+      
+      
+      congruence.
+    + (* abesr case *)
+      
+      
+
+(*
+      
+      double_pop.
+      unfold pop_stackm in *.
       rewrite <- app_assoc.
       rewrite IHil1.
       simpl.
@@ -2186,6 +1104,7 @@ Proof.
       unfold get_ev.
       monad_unfold.
       rewrite foo.
+
       (*
     rewrite <- app_assoc.
     rewrite <- IHil1.
@@ -2195,13 +1114,13 @@ Proof.
     auto.
     Unshelve. exact mtc. exact [].
       
-Defined. *)
+Defined. *) 
+*)
 Admitted.
 
 
-(*
 Lemma st_trace_destruct :
-  forall il1 il2 e s e' s',
+  forall il1 il2 e s,
     st_trace
       (fold_left run_vm_step il2
                  (fold_left run_vm_step il1
@@ -2211,99 +1130,18 @@ Lemma st_trace_destruct :
                  {| st_ev := e; st_stack := s; st_trace := [] |}) ++
       st_trace
       (fold_left run_vm_step il2
-                 {| st_ev := e';
-                    st_stack := s';
+                 {| st_ev := st_ev((fold_left run_vm_step il1 
+                 {| st_ev := e; st_stack := s; st_trace := [] |}));
+                    st_stack := st_stack((fold_left run_vm_step il1 
+                 {| st_ev := e; st_stack := s; st_trace := [] |}));
                     st_trace := [] |}).
 Proof.
   intros.
+  Check st_trace_destruct'.
   erewrite st_trace_destruct'.
-  simpl. auto.
-Defined. *)
-
-  (*
-  induction il1; (*destruct il1;*) try reflexivity; intros.
-  - simpl.
-    apply ev_irrel.
-  - simpl.
-    Check foo.
-    destruct a.
-    unfold run_vm_step. fold run_vm_step.
-    monad_unfold.
-    rewrite foo.
-    rewrite <- app_assoc.
-    rewrite <- IHil1.
-    Check foo.
-    
-    
-    rewrite app_nil_r. auto.
-  - simpl.
-    unfold run_vm_step. fold run_vm_step. destruct a. monad_unfold.
-    unfold add_tracem. monad_unfold.
-    destruct (modify_evm (prim_ev p)
-              (fold_left run_vm_step il1
-                         {| st_ev := e; st_stack := s; st_trace := [] |})).
-    destruct o.
-    + simpl.
-      Check foo.
-      assert (
-          st_trace
-            (fold_left run_vm_step il2
-               {| st_ev := prim_ev p e'; st_stack := s'; st_trace := prim_trace n p |}) =
-          prim_trace n p ++
-       st_trace
-         (fold_left run_vm_step il2
-                    {| st_ev := prim_ev p e'; st_stack := s'; st_trace := [] |})).
-      apply foo.
-      rewrite H.
-      rewrite <- foo at 3.
-      rewrite <- IHil2.
-    
-
-
-    
-    
-
-  -  destruct a.
-    destruct p; try 
-                  unfold run_vm_step; fold run_vm_step; monad_unfold;
-      eapply ev_irrel.
-
-  - simpl in *.
-    Check foo.
-    unfold run_vm_step. fold run_vm_step. monad_unfold.
-    destruct a; destruct a0. monad_unfold. unfold add_tracem.
-    unfold modify. unfold add_trace. fold add_trace.
-    monad_unfold. simpl. unfold modify_evm. monad_unfold. simpl.
-    
-
-
-    monad_unfold.
-    destruct (modify_evm (prim_ev p)
-              (fold_left run_vm_step il1
-                 {|
-                 st_ev := prim_ev p0 e;
-                 st_stack := s;
-                 st_trace := prim_trace n0 p0 |})).
-    destruct o; simpl.
-    unfold add_trace. simpl.
-    destruct v.
-    admit.
-    simpl.
-    
-    reflexivity.
-    admit.
-    rewrite <- IHil2.
-    
-
-    simpl.
-    rewrite fold_left_app.
-    simpl.
-    destruct a; destruct a0.
-    simpl.
-    rewrite <- IHil1.   
-    
-    
-Admitted. *)
+  simpl.
+  auto.
+Defined.
 
 Lemma destruct_compiled_appended : forall trd trd' il1 il2 e e'' s s'',
     run_vm
@@ -2670,13 +1508,7 @@ Proof.
       exact [].
 Admitted.
 
-Lemma push_stackm_facts : forall st_ev st_ev0 (st_trace:list Ev) (st_trace0:list Ev)
-                            st_stack st_stack0 st_trace st_trace0 H0 u,
-    (Some u, {| st_ev := st_ev0; st_stack := st_stack0; st_trace := st_trace0 |}) =
-    push_stackm H0 {| st_ev := st_ev; st_stack := st_stack; st_trace := st_trace |} ->
-    st_ev = st_ev0 /\ st_trace = st_trace0 /\ st_stack0 = H0 :: st_stack.
-Proof.
-Admitted.
+
 
 Lemma multi_stack_restore : forall t tr1 tr1' e e' s s',
     run_vm (instr_compiler t)
@@ -3262,6 +2094,172 @@ Defined.
 
 
 (******* ABANDONED PROOFS ********)
+
+
+(*
+Lemma ev_determ : forall il e s tr1 tr1' e' s' tr2,
+    fold_left run_vm_step il {| st_ev := e; st_stack := s; st_trace := tr1 |} =
+    {| st_ev := e'; st_stack := s'; st_trace := tr1' |} ->
+    st_ev (fold_left run_vm_step il {| st_ev := e; st_stack := s; st_trace := tr2 |}) = e'.
+Proof.
+  induction il; intros.
+  - simpl. simpl in H. congruence.
+  - simpl;
+    unfold run_vm_step; fold run_vm_step;
+    destruct a; try (simpl; monad_unfold;
+    try (destruct p); simpl;
+    eapply IHil; simpl in *; unfold run_vm_step in *; fold run_vm_step in H; simpl in *;
+    unfold execSt in *; simpl in *; eassumption).
+    + (* joins case *)
+      
+      unfold run_vm_step in *. fold run_vm_step in *. monad_unfold.
+      unfold run_vm_step in H. fold run_vm_step in H. monad_unfold.
+      unfold get_ev in *. monad_unfold.
+      
+
+      remember (pop_stackm {| st_ev := e; st_stack := s; st_trace := tr2 |}) as r.
+      destruct r. destruct o.
+(*
+      remember (push_stackm (ssc e0 e) v) as p.
+      destruct p. destruct o. *)
+      simpl.
+      
+      remember (pop_stackm {| st_ev := e; st_stack := s; st_trace := tr1 |}) as r.
+      destruct r. destruct o.
+(*
+      remember (push_stackm (ssc e1 e) v1) as p.
+      destruct p. destruct o. *)
+      simpl in *. monad_unfold.
+      unfold add_trace in *.
+      dependent destruction v.
+      (*dependent destruction v2.*)
+      dependent destruction v0.
+      (*dependent destruction v1. *)
+      eapply IHil.
+      assert (st_ev2 = st_ev0). {
+        assert (st_ev = st_ev0). {
+          admit. }
+        rewrite <- H0. clear Heqp0.
+        assert (st_ev1 = st_ev2). {
+          admit. }
+        rewrite <- H1.
+        assert (e = st_ev1). {
+          admit. }
+        rewrite <- H2.
+        eapply pop_stackm_pure; eauto. }
+      
+      subst.
+
+      assert (st_stack2 = st_stack0). {
+        admit. (* push/pops correspond on s *)
+      }
+      subst. eassumption.
+          
+        
+        
+      admit.
+
+
+      dependent destruction v.
+      dependent destruction v0.
+      admit.
+      admit.
+      
+
+      remember (pop_stackm {| st_ev := e; st_stack := s; st_trace := tr1 |}) as r.
+      destruct r. destruct o.
+
+      remember (push_stackm (ssc e0 e) v0) as p.
+      destruct p. destruct o.
+      dependent destruction v.
+      dependent destruction v0.
+      dependent destruction v1.
+      simpl in *.
+      admit.
+      admit.
+      simpl in *.
+      dependent destruction v.
+      dependent destruction v0.
+
+      eapply IHil.
+      assert (st_ev0 = st_ev). {
+        admit. }
+      assert (st_stack0 = st_stack). {
+        admit. }
+      subst. eassumption.
+    + (* besr case *)
+Admitted.
+*)
+
+(*
+Lemma stack_determ : forall il e s tr1 tr1' e' s' tr1'',
+    fold_left run_vm_step il {| st_ev := e; st_stack := s; st_trace := tr1 |} =
+    {| st_ev := e'; st_stack := s'; st_trace := tr1' |} ->
+    st_stack (fold_left run_vm_step il {| st_ev := e; st_stack := s; st_trace := tr1'' |}) = s'.
+Proof.
+  (*
+    induction il; intros.
+  - simpl. simpl in H. congruence.
+  - simpl;
+    unfold run_vm_step; fold run_vm_step;
+    destruct a; simpl; monad_unfold;
+    destruct p; simpl;
+    eapply IHil; simpl in *; unfold run_vm_step in *; fold run_vm_step in H; simpl in *;
+      unfold execSt in *; simpl in *; eassumption.
+
+Defined. *)
+Admitted.
+*)
+
+   (*   
+Lemma run_vm_monotonic' : forall il x x0 e s,
+    st_trace (fold_left run_vm_step il
+                        {| st_ev := e; st_trace := []; st_stack := s |}) = x0 ->
+    st_trace (fold_left run_vm_step il
+                        {| st_ev := e; st_trace := x; st_stack := s |}) = x ++ x0.
+Proof.
+  intros.
+  rewrite foo in H. simpl in H. subst.
+  rewrite foo. auto.
+Defined.
+    
+Lemma run_vm_monotonic : forall il x x0 e e' s s',
+    fold_left run_vm_step il
+              {| st_ev := e; st_trace := []; st_stack := s |} =
+    {| st_ev := e'; st_trace := x0; st_stack := s' |} ->
+    fold_left run_vm_step il
+              {| st_ev := e; st_trace := x; st_stack := s |} =
+    {| st_ev := e'; st_trace := x ++ x0; st_stack := s' |}.
+Proof.
+  intros.
+  assert (st_trace (fold_left run_vm_step il {| st_ev :=e; st_trace := x; st_stack := s |}) = x ++ x0).
+  { 
+    apply run_vm_monotonic'.
+    assert (fold_left run_vm_step il {| st_ev := e; st_trace := []; st_stack := s |} =
+            {| st_ev := e'; st_trace := x0; st_stack := s' |} ->
+            st_trace (fold_left run_vm_step il {| st_ev := e; st_trace := []; st_stack := s |}) =
+            st_trace ({| st_ev := e'; st_trace := x0; st_stack := s' |})).
+    { congruence. }
+    
+  apply H0 in H.
+  simpl in H. auto. }
+       (*      
+  assert (st_ev (fold_left run_vm_step il {| st_trace := x |}) = e').
+  eapply ev_determ. eassumption. (* TODO: ev deterministic regardless of trace, stack *)
+  assert (st_stack (fold_left run_vm_step il {| st_trace := x |}) = s).
+  eapply stack_determ. eassumption. (* TODO stack deterministic regardless of trace, ev *)
+*)
+
+  apply st_congr; eauto.
+  eapply trace_irrel; eauto.
+  eapply stack_irrel; eauto.
+Defined.
+*)
+
+
+
+
+
 
 
 (**** restIL def  *)
